Add files via upload

src.v
@@ -1,26 +1,8 @@
 Require Import Coq.Init.Nat.
 
-Definition nat_map: Type := nat -> nat.
+(* ==================== program ==================== *)
 
-Definition nat_map_empty: nat_map := (fun _ => 0).
-
-Definition nat_map_update (m: nat_map) (key: nat) (value: nat) : nat_map :=
-  fun k' => if k' =? key then value else m k'.
-
-Notation "x '!->' v" := (nat_map_update nat_map_empty x v)
-  (at level 100, v at next level, right associativity).
-
-Notation "x '!->' v ';' m" := (nat_map_update m x v)
-  (at level 100, v at next level, right associativity).
-
-Inductive program : Type :=
-  | p_single (f : function)
-  | p_cons (f : function) (p : program)
-
-with function : Type :=
-  | f_func (fn : nat) (s : statement)
-
-with statement : Type :=
+Inductive statement : Type :=
   | s_skip
   | s_cons (i : instruction) (s : statement)
 
@@ -30,37 +12,145 @@ with instruction : Type :=
   | i_while (d : nat) (s : statement)
   | i_async (s : statement)
   | i_finish (s : statement)
-  | i_call (f : function)
+  | i_call (f : nat)
 
 with expression : Type :=
   | e_const (c : nat)
   | e_add (d : nat).
 
-Inductive contains : program -> nat -> Prop :=
-  | c_single fn s : contains (p_single (f_func fn s)) fn
-  | c_hd fn s p : contains (p_cons (f_func fn s) p) fn
-  | c_tl p fn fn' s' : contains p fn -> contains (p_cons (f_func fn' s') p) fn.
+Definition program := list statement.
 
-Fixpoint find_function_body (p : program) (fn : nat) : statement :=
-  match p with
-  | p_single f => match f with
-                | f_func fn' s => if fn =? fn' then s else s_skip
-                end
-  | p_cons f p' => match f with
-                   | f_func fn' s => if fn =? fn' then s else find_function_body p' fn
-                   end
+Fixpoint concat (s1 : statement) (s2 : statement) : statement :=
+  match s1 with
+  | s_skip => s_cons i_skip s2
+  | s_cons i s => s_cons i (concat s s2)
   end.
 
-Inductive well_formed : program -> Prop := .
+Fixpoint well_formed_statement (s : statement) (n : nat) : Prop :=
+  match s with
+  | s_skip => True
+  | s_cons i s' => match i with
+                  | i_skip => well_formed_statement s' n
+                  | i_assign d e => well_formed_statement s' n
+                  | i_while d s'' => well_formed_statement s'' n /\ well_formed_statement s' n
+                  | i_async s'' => well_formed_statement s'' n /\ well_formed_statement s' n
+                  | i_finish s'' => well_formed_statement s'' n /\ well_formed_statement s' n
+                  | i_call fi => fi < n /\ well_formed_statement s' n
+                  end
+  end.
+
+Fixpoint well_formed_program (p : program) (n : nat) : Prop :=
+  match p with
+  | nil => True
+  | cons s tl => well_formed_statement s n /\ well_formed_program tl n
+  end.
+
+Fixpoint get_function_body (p : program) (n : nat) : statement :=
+  match p with
+  | nil => s_skip
+  | cons s tl => if n =? 0 then s else get_function_body tl (n - 1)
+  end.
+
+(* ==================== array ==================== *)
+
+Definition array : Type := nat -> nat.
+
+Definition empty_array : array := (fun _ => 0).
+
+Definition update_array (a : array) (key : nat) (value : nat) : array :=
+  fun k' => if k' =? key then value else a k'.
+
+Notation "x '!->' v" := (update_array empty_array x v)
+  (at level 100, v at next level, right associativity).
+
+Notation "x '!->' v ';' a" := (update_array a x v)
+  (at level 100, v at next level, right associativity).
+
+Definition eval_expression (a : array) (e : expression) : nat :=
+  match e with
+  | e_const c => c
+  | e_add d => (a d) + 1
+  end.
+
+(* ==================== tree ==================== *)
 
 Inductive tree : Type :=
   | t_ord (t1 : tree) (t2 : tree)
   | t_unord (t1 : tree) (t2 : tree)
-  | t_stat (s : statement)
-  | t_final.
+  | t_stmt (s : statement)
+  | t_finished.
 
-Inductive array : Type :=.
+Fixpoint well_formed_tree (t : tree) (n : nat) : Prop :=
+  match t with
+  | t_ord t1 t2 => well_formed_tree t1 n /\ well_formed_tree t2 n
+  | t_unord t1 t2 => well_formed_tree t1 n /\ well_formed_tree t2 n
+  | t_stmt s => well_formed_statement s n
+  | t_finished => True
+  end.
 
-Inductive steps_to : program -> array -> tree -> program -> array -> tree -> Prop := .
+(* ==================== steps-to ==================== *)
 
-Theorem progress : forall (p : program) (a : array) (t : tree), well_formed p -> t = t_final \/ exists a' t', steps_to p a t p a' t'.
+Inductive steps_to : program -> array -> tree -> program -> array -> tree -> Prop :=
+  | one p a t :
+    steps_to p a (t_ord t_finished t) p a t
+  | two p a t1 a' t1' t2 :
+    steps_to p a t1 p a' t1' ->
+    steps_to p a (t_ord t1 t2) p a' (t_ord t1' t2)
+  | three p a t2 :
+    steps_to p a (t_unord t_finished t2) p a t2
+  | four p a t1 :
+    steps_to p a (t_unord t1 t_finished) p a t1
+  | five p a t1 a' t1' t2 :
+    steps_to p a t1 p a' t1' ->
+    steps_to p a (t_unord t1 t2) p a' (t_unord t1' t2)
+  | six p a t2 a' t2' t1 :
+    steps_to p a t2 p a' t2' ->
+    steps_to p a (t_unord t1 t2) p a' (t_unord t1 t2')
+  | seven p a :
+    steps_to p a (t_stmt s_skip) p a t_finished
+  | eight p a k :
+    steps_to p a (t_stmt (s_cons i_skip k)) p a (t_stmt k)
+  | nine p a d e k :
+    steps_to p a (t_stmt (s_cons (i_assign d e) k)) p (update_array a d (eval_expression a e)) (t_stmt k)
+  | ten a d p s k :
+    a d = 0 ->
+    steps_to p a (t_stmt (s_cons (i_while d s) k)) p a (t_stmt k)
+  | eleven a d p k s :
+    a d <> 0 ->
+    steps_to p a (t_stmt (s_cons (i_while d s) k)) p a (t_stmt (concat s (s_cons (i_while d s) k)))
+  | twelve p a s k :
+    steps_to p a (t_stmt (s_cons (i_async s) k)) p a (t_unord (t_stmt s) (t_stmt k))
+  | thirteen p a s k :
+    steps_to p a (t_stmt (s_cons (i_finish s) k)) p a (t_ord (t_stmt s) (t_stmt k))
+  | fourteen p a f k :
+    steps_to p a (t_stmt (s_cons (i_call f) k)) p a (t_stmt (concat (get_function_body p f) k)).
+
+Theorem progress : forall (p : program) (a : array) (t : tree),
+  well_formed_program p (length p) ->
+  well_formed_tree t (length p) ->
+  t = t_finished \/ exists a' t', steps_to p a t p a' t'.
+Proof.
+  intros p a t H1 H2.
+  induction t; simpl.
+  - destruct IHt1.
+    + simpl in H2. apply H2.
+    + right. exists a. exists t2. subst. apply one.
+    + right. inversion H. inversion H0. exists x. exists (t_ord x0 t2). constructor. assumption.
+  - destruct IHt1.
+    + simpl in H2. apply H2.
+    + right. exists a. exists t2. subst. constructor.
+    + right. inversion H. inversion H0. exists x. exists (t_unord x0 t2). constructor. assumption.
+  - destruct s.
+    + right. exists a. exists t_finished. constructor.
+    + destruct i; right.
+      * exists a. exists (t_stmt s). constructor.
+      * exists (update_array a d (eval_expression a e)). exists (t_stmt s). constructor.
+      * exists a. assert (a d = 0 \/ a d <> 0). { destruct (a d). { left. reflexivity. } { right. discriminate. } }
+        destruct H.
+        { exists (t_stmt s). apply ten. apply H. }
+        { exists (t_stmt (concat s0 (s_cons (i_while d s0) s))). apply eleven. apply H. }
+      * exists a. exists (t_unord (t_stmt s0) (t_stmt s)). constructor.
+      * exists a. exists (t_ord (t_stmt s0) (t_stmt s)). constructor.
+      * exists a. exists (t_stmt (concat (get_function_body p f) s)). constructor.
+  - left. reflexivity.
+Qed.
